coq/Newton.v
@@ -3,12 +3,13 @@
 From Stdlib Require Import Utf8.
 From Stdlib Require Import QArith.
 
-Require Import ConvexHull.
+Require Import Misc ConvexHull.
 
 Set Implicit Arguments.
 
 Definition γ ns :=
-  (snd (ini_pt ns) - snd (fin_pt ns)) / (fst (fin_pt ns) - fst (ini_pt ns)).
+  (snd (ini_pt ns) - snd (fin_pt ns)) /
+    (Qnat (fst (fin_pt ns)) - Qnat (fst (ini_pt ns))).
 
 Definition β ns :=
-  snd (ini_pt ns) + fst (ini_pt ns) * γ ns.
+  snd (ini_pt ns) + Qnat (fst (ini_pt ns)) * γ ns.
