coq/PolyConvexHull.v
@@ -1,6 +1,6 @@
 (* PolyConvexHull.v *)
 
-From Stdlib Require Import Utf8 QArith.
+From Stdlib Require Import Utf8 Arith QArith.
 
 Require Import Misc.
 Require Import Field2.
@@ -22,7 +22,7 @@ Variable K : field r.
 Theorem points_in_any_newton_segment : ∀ f L,
   newton_segments f = Some L
   → ∀ h αh, (h, αh) ∈ [ini_pt L; fin_pt L … oth_pts L]
-    → β L == αh + h * γ L.
+    → β L == αh + Qnat h * γ L.
 Proof.
 intros f L HL h αh Hαh.
 eapply points_in_any_newton_segment₁; try eassumption; try reflexivity.
@@ -33,7 +33,7 @@ Theorem points_not_in_any_newton_segment : ∀ (f : puis_ser_pol α) pts L,
   pts = points_of_ps_polynom f
   → newton_segments f = Some L
     → ∀ h αh, (h, αh) ∈ pts ∧ (h, αh) ∉ [ini_pt L; fin_pt L … oth_pts L]
-      → β L < αh + h * (γ L).
+      → β L < αh + Qnat h * (γ L).
 Proof.
 intros f pts L Hpts HL h αh Hαhnαh.
 subst pts.
@@ -41,35 +41,27 @@ eapply points_not_in_any_newton_segment₁; try eassumption.
 eapply points_of_polyn_sorted; reflexivity.
 Qed.
 
-Theorem list_Q_pair_in_dec : ∀ a b (l : list (Q * Q)),
+Theorem list_nat_Q_pair_in_dec : ∀ a b (l : list (nat * Q)),
   {(a, b) ∈ l} + {(a, b) ∉ l}.
 Proof.
 intros a b l.
 apply List.In_dec.
 intros x y.
-destruct x as ((xan, xad), (xbn, xbd)).
-destruct y as ((yan, yad), (ybn, ybd)).
-destruct (Z.eq_dec xan yan) as [Han| Han]. {
-  subst xan.
-  destruct (Pos.eq_dec xad yad) as [Had| Had]. {
-    subst xad.
-    destruct (Z.eq_dec xbn ybn) as [Hbn| Hbn]. {
-      subst xbn.
-      destruct (Pos.eq_dec xbd ybd) as [Hbd| Hbd]. {
-        subst xbd.
-        left; reflexivity.
-      }
-      right; intros H.
-      injection H; clear H; intros; subst.
-      apply Hbd; reflexivity.
+destruct x as (x, (xbn, xbd)).
+destruct y as (y, (ybn, ybd)).
+destruct (Nat.eq_dec x y) as [Han| Han]. {
+  subst x.
+  destruct (Z.eq_dec xbn ybn) as [Hbn| Hbn]. {
+    subst xbn.
+    destruct (Pos.eq_dec xbd ybd) as [Hbd| Hbd]. {
+      now left; subst xbd.
+    } {
+      right; intros H; apply Hbd; clear Hbd.
+      now injection H.
     }
-    right; intros H.
-    injection H; clear H; intros; subst.
-    apply Hbn; reflexivity.
   }
   right; intros H.
-  injection H; clear H; intros; subst.
-  apply Had; reflexivity.
+  now injection H; clear H; intros; subst.
 }
 right; intros H.
 injection H; clear H; intros; subst.
@@ -80,11 +72,11 @@ Theorem points_in_convex : ∀ (f : puis_ser_pol α) pts L,
   pts = points_of_ps_polynom f
   → newton_segments f = Some L
     → ∀ h αh, (h, αh) ∈ pts
-      → β L <= αh + h * (γ L).
+      → β L <= αh + Qnat h * (γ L).
 Proof.
 intros f pts L Hpts HL h αh Hαh.
 remember [ini_pt L; fin_pt L … oth_pts L] as spts.
-pose proof (list_Q_pair_in_dec h αh spts) as H.
+pose proof (list_nat_Q_pair_in_dec h αh spts) as H.
 subst spts; destruct H as [H| H]. {
   eapply points_in_any_newton_segment in H; [ idtac | eassumption ].
   rewrite H; apply Qle_refl.
