coq/SlopeMisc.v
@@ -1,7 +1,7 @@
 (* SlopeMisc.v *)
 
 From Stdlib Require Import Utf8.
-From Stdlib Require Import QArith.
+From Stdlib Require Import ZArith QArith.
 
 Require Import Slope_base.
 Require Import Misc.
@@ -44,17 +44,17 @@ rewrite <- H in Heqcmp; assumption.
 Qed.
 
 Theorem slope_cmp_flatten : ∀ x₁ y₁ x₂ y₂ x₃ y₃ x₄ y₄,
-  x₁ < x₂
-  → x₃ < x₄
+  (x₁ < x₂)%nat
+  → (x₃ < x₄)%nat
     → (slope_expr (x₁, y₁) (x₂, y₂) ?= slope_expr (x₃, y₃) (x₄, y₄)) =
-      (y₂ * x₄ + y₁ * x₃ + y₃ * x₂ + y₄ * x₁ ?=
-       y₄ * x₂ + y₃ * x₁ + y₁ * x₄ + y₂ * x₃).
+      (y₂ * Qnat x₄ + y₁ * Qnat x₃ + y₃ * Qnat x₂ + y₄ * Qnat x₁ ?=
+       y₄ * Qnat x₂ + y₃ * Qnat x₁ + y₁ * Qnat x₄ + y₂ * Qnat x₃).
 Proof.
 intros x₁ y₁ x₂ y₂ x₃ y₃ x₄ y₄ Hlt₁₂ Hlt₃₄.
 unfold slope_expr; simpl.
-rewrite Qcmp_shift_mult_r; [ idtac | apply Qlt_minus; assumption ].
+rewrite Qcmp_shift_mult_r; [ idtac | apply Qlt_minus, Qnat_lt; assumption ].
 rewrite Qmult_div_swap.
-rewrite Qcmp_shift_mult_l; [ idtac | apply Qlt_minus; assumption ].
+rewrite Qcmp_shift_mult_l; [ idtac | apply Qlt_minus, Qnat_lt; assumption ].
 repeat rewrite Qmult_minus_distr_l.
 repeat rewrite Qmult_minus_distr_r.
 repeat rewrite Qminus_minus_assoc.
@@ -68,9 +68,9 @@ Qed.
 (* should use 'slope_cmp_flatten' like the other theorems, but pb with
    conditions... *)
 Theorem slope_eq : ∀ x₁ y₁ x₂ y₂ x₃ y₃,
-  ¬x₁ == x₂
-  → ¬x₂ == x₃
-    → ¬x₃ == x₁
+  x₁ ≠ x₂
+  → x₂ ≠ x₃
+    → x₃ ≠ x₁
       → slope_expr (x₁, y₁) (x₂, y₂) == slope_expr (x₁, y₁) (x₃, y₃)
         → slope_expr (x₁, y₁) (x₂, y₂) == slope_expr (x₂, y₂) (x₃, y₃).
 Proof.
@@ -82,23 +82,25 @@ apply Qeq_shift_mult_l in H. {
   apply Qeq_shift_mult_l in H. {
     apply Qeq_shift_div_l. {
       intros HH; apply H₁₂.
-      symmetry; apply Qminus_eq; assumption.
+      apply Qminus_eq, Qden_cancel in HH.
+      now apply Nat2Z.inj in HH.
     }
     symmetry.
     rewrite Qmult_div_swap.
     apply Qeq_shift_div_l. {
       intros HH; apply H₂₃.
-      symmetry; apply Qminus_eq; assumption.
+      apply Qminus_eq, Qden_cancel in HH.
+      now apply Nat2Z.inj in HH.
     }
-    setoid_replace ((y₃ - y₁) * (x₂ - x₁)) with
-     (x₂ * y₃ - x₂ * y₁ - x₁ * y₃ + x₁ * y₁) in H by ring.
-    setoid_replace ((y₂ - y₁) * (x₃ - x₁)) with
-     (x₃ * y₂ - x₃ * y₁ - x₁ * y₂ + x₁ * y₁) in H by ring.
+    setoid_replace ((y₃ - y₁) * (Qnat x₂ - Qnat x₁)) with
+     (Qnat x₂ * y₃ - Qnat x₂ * y₁ - Qnat x₁ * y₃ + Qnat x₁ * y₁) in H by ring.
+    setoid_replace ((y₂ - y₁) * (Qnat x₃ - Qnat x₁)) with
+     (Qnat x₃ * y₂ - Qnat x₃ * y₁ - Qnat x₁ * y₂ + Qnat x₁ * y₁) in H by ring.
     apply Qplus_inj_r in H.
-    setoid_replace ((y₃ - y₂) * (x₂ - x₁)) with
-     (x₁ * y₂ + x₂ * y₃ - x₁ * y₃ - x₂ * y₂) by ring.
-    setoid_replace ((y₂ - y₁) * (x₃ - x₂)) with
-     (x₂ * y₁ + x₃ * y₂ - x₃ * y₁ - x₂ * y₂) by ring.
+    setoid_replace ((y₃ - y₂) * (Qnat x₂ - Qnat x₁)) with
+     (Qnat x₁ * y₂ + Qnat x₂ * y₃ - Qnat x₁ * y₃ - Qnat x₂ * y₂) by ring.
+    setoid_replace ((y₂ - y₁) * (Qnat x₃ - Qnat x₂)) with
+     (Qnat x₂ * y₁ + Qnat x₃ * y₂ - Qnat x₃ * y₁ - Qnat x₂ * y₂) by ring.
     unfold Qminus at 1.
     unfold Qminus at 2.
     apply Qplus_inj_r.
@@ -110,84 +112,86 @@ apply Qeq_shift_mult_l in H. {
     rewrite <- Qplus_minus_swap.
     symmetry.
     apply Qeq_plus_minus_eq_r.
-    setoid_replace (x₂ * y₁ + x₃ * y₂ + x₁ * y₃) with
-     (x₃ * y₂ + x₁ * y₃ + x₂ * y₁) by ring.
+    setoid_replace (Qnat x₂ * y₁ + Qnat x₃ * y₂ + Qnat x₁ * y₃) with
+     (Qnat x₃ * y₂ + Qnat x₁ * y₃ + Qnat x₂ * y₁) by ring.
     rewrite H; ring.
   }
   intros HH; apply H₃₁.
-  apply Qminus_eq; assumption.
+  apply Qminus_eq, Qden_cancel in HH.
+  now apply Nat2Z.inj in HH.
 }
 intros HH; apply H₁₂.
-symmetry; apply Qminus_eq; assumption.
+symmetry; apply Qminus_eq, Qden_cancel in HH.
+now apply Nat2Z.inj in HH.
 Qed.
 
 Theorem slope_cmp_norm₁₂₁₃ : ∀ x₁ y₁ x₂ y₂ x₃ y₃,
-  x₁ < x₂ < x₃
+  (x₁ < x₂ < x₃)%nat
   → (slope_expr (x₁, y₁) (x₂, y₂) ?= slope_expr (x₁, y₁) (x₃, y₃)) =
-    (x₁ * y₃ + x₂ * y₁ + x₃ * y₂ ?= x₁ * y₂ + x₂ * y₃ + x₃ * y₁).
+    (Qnat x₁ * y₃ + Qnat x₂ * y₁ + Qnat x₃ * y₂ ?= Qnat x₁ * y₂ + Qnat x₂ * y₃ + Qnat x₃ * y₁).
 Proof.
 intros x₁ y₁ x₂ y₂ x₃ y₃ (Hlt₁, Hlt₂).
-assert (x₁ < x₃) as Hlt₃ by (eapply Qlt_trans; eassumption).
+assert (x₁ < x₃)%nat as Hlt₃ by (eapply Nat.lt_trans; eassumption).
 rewrite slope_cmp_flatten; [ idtac | assumption | assumption ].
 rewrite <- Qplus_assoc, Qplus_comm, Qplus_assoc.
-remember (y₁ * x₂ + y₃ * x₁ + y₂ * x₃ + y₁ * x₁) as t.
+remember (y₁ * Qnat x₂ + y₃ * Qnat x₁ + y₂ * Qnat x₃ + y₁ * Qnat x₁) as t.
 rewrite <- Qplus_assoc, Qplus_comm, Qplus_assoc; subst t.
 rewrite <- Qplus_cmp_compat_r.
-setoid_replace (y₁ * x₂ + y₃ * x₁ + y₂ * x₃) with
- (x₁ * y₃ + x₂ * y₁ + x₃ * y₂) by ring.
-setoid_replace (y₁ * x₃ + y₂ * x₁ + y₃ * x₂) with
- (x₁ * y₂ + x₂ * y₃ + x₃ * y₁) by ring.
+setoid_replace (y₁ * Qnat x₂ + y₃ * Qnat x₁ + y₂ * Qnat x₃) with
+ (Qnat x₁ * y₃ + Qnat x₂ * y₁ + Qnat x₃ * y₂) by ring.
+setoid_replace (y₁ * Qnat x₃ + y₂ * Qnat x₁ + y₃ * Qnat x₂) with
+ (Qnat x₁ * y₂ + Qnat x₂ * y₃ + Qnat x₃ * y₁) by ring.
 reflexivity.
 Qed.
 
 Theorem slope_cmp_norm₁₃₁₂ : ∀ x₁ y₁ x₂ y₂ x₃ y₃,
-  x₁ < x₂ < x₃
+  (x₁ < x₂ < x₃)%nat
   → (slope_expr (x₁, y₁) (x₃, y₃) ?= slope_expr (x₁, y₁) (x₂, y₂)) =
-    (x₁ * y₂ + x₂ * y₃ + x₃ * y₁ ?= x₁ * y₃ + x₂ * y₁ + x₃ * y₂).
+    (Qnat x₁ * y₂ + Qnat x₂ * y₃ + Qnat x₃ * y₁ ?= Qnat x₁ * y₃ + Qnat x₂ * y₁ + Qnat x₃ * y₂).
 Proof.
 intros; apply Qcmp_sym, slope_cmp_norm₁₂₁₃; assumption.
 Qed.
 
 Theorem slope_cmp_norm₁₃₂₃ : ∀ x₁ y₁ x₂ y₂ x₃ y₃,
-  x₁ < x₂ < x₃
+  (x₁ < x₂ < x₃)%nat
   → (slope_expr (x₁, y₁) (x₃, y₃) ?= slope_expr (x₂, y₂) (x₃, y₃)) =
-    (x₁ * y₃ + x₂ * y₁ + x₃ * y₂ ?= x₁ * y₂ + x₂ * y₃ + x₃ * y₁).
+    (Qnat x₁ * y₃ + Qnat x₂ * y₁ + Qnat x₃ * y₂ ?= Qnat x₁ * y₂ + Qnat x₂ * y₃ + Qnat x₃ * y₁).
 Proof.
 intros x₁ y₁ x₂ y₂ x₃ y₃ (Hlt₁, Hlt₂).
-assert (x₁ < x₃) as Hlt₃ by (eapply Qlt_trans; eassumption).
+assert (x₁ < x₃)%nat as Hlt₃ by (eapply Nat.lt_trans; eassumption).
 rewrite slope_cmp_flatten; [ idtac | assumption | assumption ].
 repeat rewrite <- Qplus_assoc.
 rewrite <- Qplus_cmp_compat_l.
 repeat rewrite Qplus_assoc.
-setoid_replace (y₁ * x₂ + y₂ * x₃ + y₃ * x₁) with
- (x₁ * y₃ + x₂ * y₁ + x₃ * y₂) by ring.
-setoid_replace (y₂ * x₁ + y₁ * x₃ + y₃ * x₂) with
- (x₁ * y₂ + x₂ * y₃ + x₃ * y₁) by ring.
+setoid_replace (y₁ * Qnat x₂ + y₂ * Qnat x₃ + y₃ * Qnat x₁) with
+ (Qnat x₁ * y₃ + Qnat x₂ * y₁ + Qnat x₃ * y₂) by ring.
+setoid_replace (y₂ * Qnat x₁ + y₁ * Qnat x₃ + y₃ * Qnat x₂) with
+ (Qnat x₁ * y₂ + Qnat x₂ * y₃ + Qnat x₃ * y₁) by ring.
 reflexivity.
 Qed.
 
 Theorem slope_cmp_norm₂₃₁₃ : ∀ x₁ y₁ x₂ y₂ x₃ y₃,
-  x₁ < x₂ < x₃
+  (x₁ < x₂ < x₃)%nat
   → (slope_expr (x₂, y₂) (x₃, y₃) ?= slope_expr (x₁, y₁) (x₃, y₃)) =
-    (x₁ * y₂ + x₂ * y₃ + x₃ * y₁ ?= x₁ * y₃ + x₂ * y₁ + x₃ * y₂).
+    (Qnat x₁ * y₂ + Qnat x₂ * y₃ + Qnat x₃ * y₁ ?= Qnat x₁ * y₃ + Qnat x₂ * y₁ + Qnat x₃ * y₂).
 Proof.
 intros; apply Qcmp_sym, slope_cmp_norm₁₃₂₃; assumption.
 Qed.
 
 Theorem slope_cmp₂ : ∀ pt₁ pt₂ pt₃,
-  fst pt₁ < fst pt₂ < fst pt₃
+  (fst pt₁ < fst pt₂ < fst pt₃)%nat
   → (slope_expr pt₁ pt₃ ?= slope_expr pt₁ pt₂) =
     (slope_expr pt₂ pt₃ ?= slope_expr pt₁ pt₃).
 Proof.
 intros (x₁, y₁) (x₂, y₂) (x₃, y₃) (Hlt₁, Hlt₂).
-assert (x₁ < x₃) as Hlt₃ by (eapply Qlt_trans; eassumption).
+assert (x₁ < x₃)%nat as Hlt₃ by (eapply Nat.lt_trans; eassumption).
 rewrite slope_cmp_norm₁₃₁₂; [ idtac | split; assumption ].
 rewrite slope_cmp_norm₂₃₁₃; [ idtac | split; assumption ].
 reflexivity.
 Qed.
 
 Theorem slope_lt_1312_2313 : ∀ pt₁ pt₂ pt₃,
-  fst pt₁ < fst pt₂ < fst pt₃
+  (fst pt₁ < fst pt₂ < fst pt₃)%nat
   → slope_expr pt₁ pt₃ < slope_expr pt₁ pt₂
     → slope_expr pt₂ pt₃ < slope_expr pt₁ pt₃.
 Proof.
