coq/Slope_base.v
@@ -4,4 +4,4 @@ From Stdlib Require Import Utf8.
 From Stdlib Require Import QArith.
 
 Definition slope_expr pt₁ pt₂ :=
-  (snd pt₂ - snd pt₁) / (fst pt₂ - fst pt₁).
+  (snd pt₂ - snd pt₁) / ((Z.of_nat (fst pt₂) # 1) - (Z.of_nat (fst pt₁) # 1)).
